Working models of map and from_fn for arrays.

hax-lib/proof-libs/fstar/core/Core_models.Array.fst
@@ -5,24 +5,11 @@ open Rust_primitives
 
 type t_TryFromSliceError = | TryFromSliceError : t_TryFromSliceError
 
-let impl_23__map
-      (#v_T: Type0)
-      (v_N: usize)
-      (#v_U #v_F: Type0)
-      (#[FStar.Tactics.Typeclasses.tcresolve ()] i0: Core_models.Ops.Function.t_FnOnce v_F v_T)
-      (#_: unit{i0.Core_models.Ops.Function.f_Output == v_U})
-      (s: t_Array v_T v_N)
-      (f: v_F)
-    : t_Array v_U v_N = Rust_primitives.Slice.array_map #v_T #v_U v_N #v_F s f
+let impl_23__map (#v_T: Type0) (v_N: usize) (#v_U: Type0) (s: t_Array v_T v_N) (f: (v_T -> v_U))
+    : t_Array v_U v_N = Rust_primitives.Slice.array_map #v_T #v_U v_N s f
 
 let impl_23__as_slice (#v_T: Type0) (v_N: usize) (s: t_Array v_T v_N) : t_Slice v_T =
   Rust_primitives.Slice.array_as_slice #v_T v_N s
 
-let from_fn
-      (#v_T: Type0)
-      (v_N: usize)
-      (#v_F: Type0)
-      (#[FStar.Tactics.Typeclasses.tcresolve ()] i0: Core_models.Ops.Function.t_FnOnce v_F usize)
-      (#_: unit{i0.Core_models.Ops.Function.f_Output == v_T})
-      (f: v_F)
-    : t_Array v_T v_N = Rust_primitives.Slice.array_from_fn #v_T v_N #v_F f
+let from_fn (#v_T: Type0) (v_N: usize) (f: (usize -> v_T)) : t_Array v_T v_N =
+  Rust_primitives.Slice.array_from_fn #v_T v_N f
