hax-lib/proof-libs/fstar/rust_primitives/Rust_primitives.Slice.fsti
@@ -8,13 +8,10 @@ let length (#a: Type) (s: t_Slice a): res: usize {res == sz (Seq.length s)} = sz
 let split_at (#v_T: Type0) (s: t_Slice v_T) (mid: usize {mid <=. length s}): t_Slice v_T & t_Slice v_T = 
   Seq.slice s 0 (v mid), Seq.slice s (v mid) (Seq.length s)
 let slice_index (#t: Type) (s: t_Slice t) (i: usize {i <. length s}): t = Seq.index s (v i)
-let array_map (#t: Type) (#u: Type) (l: usize) (#v_F: Type) (#[FStar.Tactics.Typeclasses.tcresolve ()] i0: Core_models.Ops.Function.t_FnOnce v_F t)
-  (#_: unit{i0.Core_models.Ops.Function.f_Output == u})
-  (s: t_Array t l) (f: v_F): t_Array u l =
-  Rust_primitives.Arrays.map_array s (Core_models.Ops.Function.f_call_once f)
+val array_map (#t: Type) (#u: Type) (l: usize)
+  (s: t_Array t l) (f: t -> u): res: t_Array u l {forall i. Seq.index res i == f (Seq.index s i)}
 let array_as_slice (#t: Type) (l: usize) (s: t_Array t l): t_Slice t =
   s
-val array_from_fn (#t: Type) (len: usize) (#v_F: Type) (#[FStar.Tactics.Typeclasses.tcresolve ()] i0: Core_models.Ops.Function.t_FnOnce v_F usize)
-  (#_: unit{i0.Core_models.Ops.Function.f_Output == t}) (f: v_F): 
-  Pure (t_Array t len) (requires True) (ensures (fun a -> forall i. Seq.index a i == Core_models.Ops.Function.f_call_once f (sz i)))
+val array_from_fn (#t: Type) (len: usize) (f: usize -> t): 
+  Pure (t_Array t len) (requires True) (ensures (fun a -> forall i. Seq.index a i == f (sz i)))
 
